Update F*, tweak a few proofs

dist/Kuiper_Example_Array1.cu
@@ -1,11 +1,6 @@
 
 #include "Kuiper_Example_Array1.h"
 
-void Kuiper_Example_Array1_test0(uint32_t *m)
-{
-    KRML_MAYBE_UNUSED_VAR(m);
-}
-
 uint32_t Kuiper_Example_Array1_test1(uint32_t *m)
 {
     return m[1U];
