dist/Kuiper_Example_Array1.h
@@ -4,8 +4,6 @@
 
 #include <kuiper.h>
 
-void Kuiper_Example_Array1_test0(uint32_t * m);
-
 uint32_t Kuiper_Example_Array1_test1(uint32_t * m);
 
 void Kuiper_Example_Array1_test2(uint32_t * m);
